Fixed hbeq, added concurrent children condition

history.fst
@@ -11,24 +11,36 @@ type history (n:nat) =
             -> children:list (I.trace * history n)
             -> history n
 
-
-val hbeq : #n:nat -> h1:history n -> h2:history n -> Tot bool (decreases %[h1]) 
-val hbeq' : #n:nat -> l:list (I.trace * history n) -> h2:history n -> Tot bool (decreases %[l])
-let rec hbeq #n h1 h2 =
+(*Returns true if h1 happens before h2*)
+val hb : #n:nat -> h1:history n -> h2:history n -> Tot bool (decreases %[h1]) 
+val hb' : #n:nat -> l:list (I.trace * history n) -> s:state -> h2:history n -> Tot bool (decreases %[l])
+let rec hb #n h1 h2 =
   let History s ch = h1 in 
-  h1 = h2 || hbeq' #n ch h2 
-and hbeq' #n children h2 =
+  hb' #n ch s h2 
+and hb' #n children par_state h2 =
   match children with
-  |[] -> false
-  |(tr,x)::xs -> hbeq #n x h2 || hbeq' #n xs h2
+  | [] -> false
+  | (tr,x)::xs -> x = h2 ||
+                hb #n x h2 ||
+                hb' #n xs par_state h2
   
 
 val eq : #n:nat -> h1:history n -> h2:history n -> Tot bool (decreases %[h1]) 
 let eq #n h1 h2 = (h1 = h2)
 
-val hb : #n:nat -> h1:history n -> h2:history n -> Tot bool (decreases %[h1])
-let hb #n h1 h2 = hbeq h1 h2 && not(eq h1 h2)
+(*Returns true if h1 happens before or equal to h2*)
+val hbeq : #n:nat -> h1:history n -> h2:history n -> Tot bool (decreases %[h1])
+let hbeq #n h1 h2 = hb h1 h2 || eq h1 h2
+
+val concurrent : #n:nat -> h1:history n -> h2:history n -> Tot bool (decreases %[h1])
+let concurrent #n h1 h2 = not (hbeq h1 h2 || hbeq h2 h1)
           
+val concurrent_commutative : #n:nat 
+                             -> h1:history n 
+                             -> h2:history n{concurrent h1 h2}
+                             -> Lemma (ensures (concurrent h2 h1))
+let concurrent_commutative #n h1 h2 = ()
+
 
 val size : #n:nat -> h:history n -> Tot nat (decreases %[h])
 val size' : #n:nat -> l:list (I.trace * history n) -> Tot nat (decreases %[l])
@@ -39,32 +51,59 @@ and size' #n l =
     match l with
     | [] -> 0
     | (tr,x)::xs -> size x + size' xs
-    
 
-val wellformed : #n:nat -> h:history n -> Tot bool (decreases %[h])
-val wellformed' : #n:nat -> s:state -> l:list (I.trace * history n) -> h:history n -> Tot bool (decreases %[l])
+
+(*Returns true if all the children of a parent node are concurrent*)
+val concur_ch : #n:nat -> l:list(I.trace * history n) -> Tot bool (decreases %[l])
+val concur_ch' : #n:nat -> child:history n -> l:list(I.trace * history n) -> Tot bool (decreases %[l])
+let rec concur_ch #n l = 
+match l with 
+  |[] -> true
+  |(tr,x)::xs -> concur_ch' x xs && concur_ch xs
+and concur_ch' #n x ch =
+match ch with
+  |[] -> true
+  |(tr,y)::xs -> concurrent x y && concur_ch' x xs
+
+
+val wellformed : #n:nat -> h:history n -> Tot bool (decreases h)
+val wellformed' : #n:nat -> s:state -> l:list (I.trace * history n) -> h:history n -> Tot bool (decreases l)
 let rec wellformed #n h =
   let History state ch = h in
+  concur_ch #n ch &&
   wellformed' state ch h
-and wellformed' #n parent_state children parent_history =
+and wellformed' #n par_state children par_history =
   match children with
-  |[] -> true
-  |(tr,child_history)::xs -> 
-    let state = History?.state child_history in
-    state = I.apply_tr tr parent_state &&
-    hb parent_history child_history &&
-    wellformed child_history &&
-    wellformed' parent_state xs parent_history
+  | [] -> true
+  | (tr,ch_history)::xs -> 
+         let ch_state = History?.state ch_history in
+         hb par_history ch_history &&
+         ch_state = I.apply_tr tr par_state &&
+         wellformed ch_history &&
+         wellformed' par_state xs par_history
+    
 
 val test : #n:nat -> Tot unit
-let test #n = assert (hbeq #n (History 1 [([I.Inc;I.Inc], (History 3 [([I.Inc],(History 4 []))]))]) (History 3 [([I.Inc],(History 4 []))]));()
+let test #n = assert (hbeq #n (History 1 [([I.Inc 1;I.Inc 1], (History 3 [([I.Inc 1],(History 4 []))]))]) (History 3 [([I.Inc 1],(History 4 []))]));()
 
 val test1 : #n:nat -> Tot unit
-let test1 #n = assert (hb #n (History 1 [([I.Inc;I.Inc], (History 3 [([I.Inc],(History 4 []))]))]) (History 4 []));()
+let test1 #n = assert (hb #n (History 1 [([I.Inc 1;I.Inc 1], (History 3 [([I.Inc 1],(History 4 []))]))]) (History 4 []));()
 
 val test2 : #n:nat -> Tot unit
-let test2 #n = assert (eq #n (History 1 [([I.Inc;I.Inc], (History 3 [([I.Inc],(History 4 []))]))]) (History 1 [([I.Inc;I.Inc], (History 3 [([I.Inc],(History 4 []))]))]));()
+let test2 #n = assert (eq #n (History 1 [([I.Inc 1;I.Inc 1], (History 3 [([I.Inc 1],(History 4 []))]))]) (History 1 [([I.Inc 1;I.Inc 1], (History 3 [([I.Inc 1],(History 4 []))]))]));()
 
 
+val hbeq_reflexive : #n:nat 
+                     -> h:history n 
+                     -> Lemma (ensures (hbeq h h))
+let hbeq_reflexive #n h = ()
 
 
+val lemma1 : #n:nat 
+             -> h:history n{wellformed h}
+             -> Lemma (ensures (forall h'. hb h h' ==> wellformed h'))  (decreases (size h))
+                       
+let rec lemma1 #n (History s ch) = match ch with
+ | [] -> ()
+ | (tr,x)::xs -> lemma1 x; lemma1 (History s xs)
+          
